Equivs done

proof/spec/XMSS_vs_XMSS_MT.ec
@@ -1,56 +1,122 @@
 from Jasmin require import JModel.
-require import XMSS_PRF XMSS_MT_PRF IntDiv XMSS_Params XMSS_MT_Params Int Ring XMSS_Address  XMSS_MT_Address Array8.
+require import List DList IntDiv Int Ring.
+require import Address Hash XMSS_Params  XMSS_Types  XMSS_TreeHash XMSS_PRF  XMSS_MT_Params XMSS_MT_TreeHash XMSS_MT_Types XMSS_MT_PRF.
 import IntID.
 
-equiv keygen : XMSS_PRF.kg ~ XMSS_MT_PRF.kg : d = 1 ==> ={res}. 
+require import Array8.
+
+abbrev eqsk (sk : xmss_sk, skmt : xmss_mt_sk) : bool = 
+    sk.`idx = skmt.`idx /\
+    sk.`sk_seed = skmt.`sk_seed /\
+    sk.`sk_prf = skmt.`sk_prf /\
+    sk.`pub_seed_sk = skmt.`pub_seed_sk /\
+    sk.`sk_root = skmt.`sk_root. 
+
+abbrev eqpk (pk : xmss_pk, pkmt : xmss_mt_pk) : bool = 
+    pk.`pk_oid = pkmt.`pk_oid /\
+    pk.`pk_root = pkmt.`pk_root /\
+    pk.`pk_pub_seed = pkmt.`pk_pub_seed. 
+
+abbrev eqkp (kp : xmss_keypair, kpmt : xmss_mt_keypair) : bool = 
+    kp.`1.`idx = kpmt.`1.`idx /\
+    kp.`1.`sk_seed = kpmt.`1.`sk_seed /\
+    kp.`1.`sk_prf = kpmt.`1.`sk_prf /\
+    kp.`1.`pub_seed_sk = kpmt.`1.`pub_seed_sk /\
+    kp.`1.`sk_root = kpmt.`1.`sk_root /\
+    kp.`2.`pk_oid = kpmt.`2.`pk_oid /\
+    kp.`2.`pk_root = kpmt.`2.`pk_root /\
+    kp.`2.`pk_pub_seed = kpmt.`2.`pk_pub_seed. 
+
+
+equiv keygen : XMSS_PRF.kg ~ XMSS_MT_PRF.kg : XMSS_Params.impl_oid = XMSS_MT_Params.impl_oid /\ d = 1 ==> eqkp res{1} res{2}. 
 proof. 
-proc; inline *; sim.
-by auto => /> /#. 
+proc. wp 11 11 => /=. 
+call(:d=1);1: by conseq />; sim; auto => /> /#.
+wp 9 9 => /=. 
+call(:d=1);1: by conseq />; sim. 
+by auto => /> /#.
 qed.
 
-equiv sign : XMSS_PRF.sign ~ XMSS_MT_PRF.sign : d=1 /\ h < 32 /\ 0 < to_uint sk{2}.`Types.idx < 2^h - 1 /\ ={arg} ==> ={res}. 
+abbrev eqsig(sig : XMSS_Types.sig_t, sigmt : XMSS_MT_Types.sig_t) : bool =
+   sig.`sig_idx = sigmt.`sig_idx /\
+   sig.`r = sigmt.`r /\
+   sig.`r_sigs = sigmt.`r_sigs.
+
+equiv sign : XMSS_PRF.sign ~ XMSS_MT_PRF.sign : 
+    XMSS_Params.impl_oid = XMSS_MT_Params.impl_oid /\  
+    d=1 /\ 
+    h < 32 /\ 0 < to_uint sk{2}.`idx < 2^h - 1 /\ 
+    eqsk arg{1}.`1 arg{2}.`1 /\ arg{1}.`2 = arg{2}.`2 ==> 
+     eqsig res{1}.`1 res{2}.`1 /\ eqsk res{1}.`2 res{2}.`2. 
 proof. 
-proc. 
-rcondf {2} 24.
+proc => /=. 
+rcondf {2} 22.
 + move => ?.
   wp;call(:true);1:by trivial.
   wp;call(:true);1:by trivial.
   by auto => /> /#.
-wp;call(: true); 1: by sim.
-wp;call(: true); 1: by sim.
-auto => /> &2 => ->; rewrite !divz1 /=.
-move => *; do split.
-+ rewrite W32.and_mod /=;1:smt(ge0_h).
-  by rewrite modz_small /=; 1:smt().
 
-rewrite to_uint_shr;1:smt(ge0_h).
-rewrite /zero_address /set_tree_addr /set_layer_addr /=.
-have -> : (to_uint sk{2}.`Types.idx %/ 2 ^ h) = 0 by smt().
-apply tP => i ib.
-rewrite !initiE 1:/# /=.
-rewrite !get_setE 1..3:/#.
-by rewrite initiE 1:/# /=.
+wp => /=. 
+call(: d=1 /\ ={arg} /\ 0 < to_uint idx{1} /\ to_uint idx{2} < 2 ^ h - 1 ==> ={res}).
++ proc. 
+  call(: d=1  /\ ={arg} ==> ={res}).
+  + by proc => /=; sim. 
+  wp => /=. 
+  call(: d=1 /\ ={arg} /\ 0 < to_uint idx{1} /\ to_uint idx{2} < 2 ^ h - 1 ==> ={res}).
+  +  proc => /=. 
+     while (#post /\ d = 1 /\ ={pub_seed,sk_seed,t,j,idx} /\ 0 <= j{1} <= h /\
+       0 < to_uint idx{1} /\ to_uint idx{2} < 2 ^ h - 1).
+     + auto => />;conseq (: ={j,t,address}). smt(). 
+     call(:d=1); 1: by conseq />;sim;auto => /> /#.
+     by auto => />.
+   by auto => />;1: by smt(ge0_h).
+by auto => />.
 
+wp;call(:true); 1: by sim.
+auto => /> &1 &2 ? -> /= *;split;1:smt(). 
+move => *; do split;1: smt(). 
++ rewrite and_mod;1:smt(ge0_h).
+  by rewrite modz_small /=; smt(). 
++ rewrite /zero_address /set_tree_addr /set_layer_addr  to_uint_shr /=; 1: by smt(ge0_h). 
+  have -> : (to_uint sk{2}.`idx %/ 2 ^ h) = 0 by smt().
+  apply tP => i ib.
+  rewrite !initiE 1:/# /=.
+  rewrite !get_setE 1..3:/#.
+  by rewrite initiE 1:/# /=.
+
++ by smt().
+
++ rewrite and_mod;1:smt(ge0_h).
+  by rewrite modz_small /=; smt(). 
+
+by smt().
 qed.
 
-equiv verify : XMSS_PRF.verify ~ XMSS_MT_PRF.verify : d=1 /\ h < 32 /\ 0 < to_uint s{2}.`Types.sig_idx < 2^h - 1 /\ ={arg} ==> ={res}. 
-proof. 
-proc. 
+equiv verify : XMSS_PRF.verify ~ XMSS_MT_PRF.verify : 
+    d=1 /\ 
+    h < 32 /\ 0 < to_uint s{2}.`sig_idx < 2^h - 1 /\ 
+    eqpk arg{1}.`1 arg{2}.`1 /\ arg{1}.`2 = arg{2}.`2 /\ eqsig arg{1}.`3 arg{2}.`3 ==> ={res}.
+proc.
 rcondf {2} 16.
 + move => ?.
   wp;call(:true);1:by trivial.
   by auto => /> /#.
 wp;call(: true); 1: by sim.
-auto => /> &2 => ->; rewrite !divz1 /=.
+auto => /> &1 &2 -> /=.
 move => *; do split.
 + rewrite W32.and_mod /=;1:smt(ge0_h).
   by rewrite modz_small /=; 1:smt().
++ by smt().
++ by smt().
++ by smt().
 
-rewrite to_uint_shr;1:smt(ge0_h).
-rewrite /zero_address /set_tree_addr /set_layer_addr /=.
-have -> : (to_uint s{2}.`Types.sig_idx %/ 2 ^ h) = 0 by smt().
-apply tP => i ib.
-rewrite !initiE 1:/# /=.
-rewrite !get_setE 1..3:/#.
-by rewrite initiE 1:/# /=.
++ rewrite to_uint_shr;1:smt(ge0_h).
+  rewrite /zero_address /set_tree_addr /set_layer_addr /=.
+  have -> : (to_uint s{2}.`sig_idx %/ 2 ^ h) = 0 by smt().
+  apply tP => i ib.
+  rewrite !initiE 1:/# /=.
+  rewrite !get_setE 1..3:/#.
+  by rewrite initiE 1:/# /=.
+
+by smt().
 qed.
