proof/spec/LTree.ec
@@ -62,3 +62,19 @@ module LTree = {
 
 lemma ltree_ll : islossless LTree.ltree.
 admitted.
+
+(******************************************************************************)
+
+(* Stack operations *)
+op push (x : 'a list) (a : 'a) : 'a list = rcons x a. 
+
+op remove_last (x : 'a list) : 'a list = 
+with x = [] => []
+with x = h::t => if t = [] then [] else remove_last t.
+
+op pop (x : 'a list) : 'a list * 'a = 
+    let last_elem = last witness x in
+    let new_list = remove_last x in
+    (new_list, last_elem).
+
+(******************************************************************************)
