proof/spec/xmss/XMSS_TreeHash.ec
@@ -16,22 +16,6 @@ pred leftmost_leaf (s t : int)  = s %% 2^t = 0.
 (* Precondition *)
 pred treehash_p (s t : int) = s %% (1 `<<` t) <> 0.
 
-(******************************************************************************)
-
-(* Stack operations *)
-op push (x : 'a list) (a : 'a) : 'a list = rcons x a. 
-
-op remove_last (x : 'a list) : 'a list = 
-with x = [] => []
-with x = h::t => if t = [] then [] else remove_last t.
-
-op pop (x : 'a list) : 'a list * 'a = 
-    let last_elem = last witness x in
-    let new_list = remove_last x in
-    (new_list, last_elem).
-
-(******************************************************************************)
-
 
 (* NOTE: In the Jasmin implementation, treehash (in xmss_core.c) computes both the authentication 
          path and the resulting root node *)
